# baseURI: https://linked.data.gov.au/def/auspix
# imports: https://linked.data.gov.au/def/geox
# prefix: apo

@prefix apo: <https://linked.data.gov.au/def/auspix#> .
@prefix auspix: <http://pid.geoscience.gov.au/dggs/ausPIX/> .
@prefix data: <https://linked.data.gov.au/def/datatype/> .
@prefix dcterms: <http://purl.org/dc/terms/> .
@prefix geo: <http://www.opengis.net/ont/geosparql#> .
@prefix geox: <https://linked.data.gov.au/def/geox#> .
@prefix owl: <http://www.w3.org/2002/07/owl#> .
@prefix rdf: <http://www.w3.org/1999/02/22-rdf-syntax-ns#> .
@prefix rdfs: <http://www.w3.org/2000/01/rdf-schema#> .
@prefix sdo: <https://schema.org/> .
@prefix skos: <http://www.w3.org/2004/02/skos/core#> .
@prefix xsd: <http://www.w3.org/2001/XMLSchema#> .

<https://linked.data.gov.au/org/csiro>
  a sdo:Organization ;
  sdo:identifier <https://ror.org/03qn8fb07> ;
  sdo:mainEntityOfPage <https://www.csiro.au/> ;
  sdo:name "CSIRO" ;
.
<https://linked.data.gov.au/def/auspix>
  a owl:Ontology ;
  dcterms:created "2020-02-05"^^xsd:date ;
  dcterms:creator <https://orcid.org/0000-0002-3884-3420> ;
  dcterms:license <https://creativecommons.org/publicdomain/zero/1.0/> ;
  dcterms:modified "2020-06-02"^^xsd:date ;
  rdfs:comment """An ontology to allow AusPIX objects to be linked into Loc-I. 

Two classes are defined: a `AusPIX CellAggregate` is composed of one or more `AusPIX Cells`. 

An AusPIX CellAggregate may be used to provide a geometrical approximation for other Loc-I Features using the (loci|apo):equivalent predicate. 

![](./images/auspix.png)""" ;
  rdfs:label "AusPIX Ontology" ;
  rdfs:seeAlso <http://www.opengis.net/doc/AS/dggs/1.0> ;
  rdfs:seeAlso <https://github.com/GeoscienceAustralia/AusPIX_DGGS> ;
  owl:imports <https://linked.data.gov.au/def/geox> ;
.
apo:Cell
  a owl:Class ;
  rdfs:comment """Cell, from [AusPIX](https://github.com/GeoscienceAustralia/AusPIX-DGGS-dataset)

Individual cells should be refered to using an IRI, typically a call to the AusPIX service.""" ;
  rdfs:label "AusPIX Cell" ;
  rdfs:subClassOf geo:Feature ;
  rdfs:subClassOf [
      a owl:Restriction ;
      owl:allValuesFrom apo:Cell ;
      owl:onProperty apo:hasNeighbourDown ;
    ] ;
  rdfs:subClassOf [
      a owl:Restriction ;
      owl:allValuesFrom apo:Cell ;
      owl:onProperty apo:hasNeighbourLeft ;
    ] ;
  rdfs:subClassOf [
      a owl:Restriction ;
      owl:allValuesFrom apo:Cell ;
      owl:onProperty apo:hasNeighbourRight ;
    ] ;
  rdfs:subClassOf [
      a owl:Restriction ;
      owl:allValuesFrom apo:Cell ;
      owl:onProperty apo:hasNeighbourUp ;
    ] ;
  rdfs:subClassOf [
      a owl:Restriction ;
      owl:cardinality "1"^^xsd:nonNegativeInteger ;
      owl:onProperty geox:hasCentroid ;
    ] ;
  rdfs:subClassOf [
      a owl:Restriction ;
      owl:minCardinality "1"^^xsd:nonNegativeInteger ;
      owl:onProperty geox:hasArea ;
    ] ;
  rdfs:subClassOf [
      a owl:Restriction ;
      owl:minCardinality "1"^^xsd:nonNegativeInteger ;
      owl:onProperty dcterms:identifier ;
    ] ;
  rdfs:subClassOf [
      a owl:Restriction ;
      owl:minCardinality "1"^^xsd:nonNegativeInteger ;
      owl:onProperty geo:hasGeometry ;
    ] ;
  rdfs:subClassOf [
      a owl:Restriction ;
      owl:minCardinality "1"^^xsd:nonNegativeInteger ;
      owl:onProperty geo:sfWithin ;
    ] ;
  rdfs:subClassOf [
      a owl:Restriction ;
      owl:minCardinality "9"^^xsd:nonNegativeInteger ;
      owl:onProperty geo:sfContains ;
    ] ;
  skos:example """
auspix:R7852 a apo:Cell ;
  dcterms:identifier 'R7852' ;
  apo:hasNeighbourUp auspix:R7828 ;
  apo:hasNeighbourDown auspix:R7855 ;
  apo:hasNeighbourRight auspix:R8630 ;
  apo:hasNeighbourLeft auspix:R7851 ;
  geo:hasGeometry 'POLYGON ((148.88888888888889 -34.663795228918765, 150.0 -34.663795228918765, 150.0 -35.81859718358464, 148.88888888888889 -35.81859718358464))'^^geo:wktLiteral ;
  geo:sfContains auspix:R78520 , auspix:R78521 , auspix:R78522 , auspix:R78523 , auspix:R78524 , auspix:R78525 , auspix:R78526 , auspix:R78527 , auspix:R78528 ; 
  geo:sfWithin auspix:R785 ; 
  geox:hasCentroid 'POINT (149.44444444444443 -35.23915910922053)'^^geo:wktLiteral ;
  geox:hasAreaM2 [ data:value 12971551595.0 ] ; 
.""" ;
.
apo:CellAggregate
  a owl:Class ;
  rdfs:comment "An AusPIX CellAggregate is composed of a set of auspix Cells" ;
  rdfs:label "AusPIX CellAggregate" ;
  rdfs:subClassOf geo:Feature ;
  rdfs:subClassOf [
      a owl:Restriction ;
      owl:allValuesFrom apo:Cell ;
      owl:onProperty rdfs:member ;
    ] ;
  rdfs:subClassOf [
      a owl:Restriction ;
      owl:minCardinality "1"^^xsd:nonNegativeInteger ;
      owl:onProperty rdfs:member ;
    ] ;
  skos:example """
auspix:Agg_1
  rdf:type apo:CellAggregate ;
  dcterms:identifier 'Agg_1' ;
  rdfs:member auspix:R7828 ;
  rdfs:member auspix:R78520 ;
  rdfs:member auspix:R78521 ;
  rdfs:member auspix:R78522 ;
  rdfs:member auspix:R78523 ;
.""" ;
.
apo:hasNeighbourDown
  a owl:ObjectProperty ;
  rdfs:label "has neighbour downward" ;
  rdfs:subPropertyOf geo:sfTouches ;
.
apo:hasNeighbourLeft
  a owl:ObjectProperty ;
  rdfs:label "has neighbour to the left" ;
  rdfs:subPropertyOf geo:sfTouches ;
.
apo:hasNeighbourRight
  a owl:ObjectProperty ;
  rdfs:label "has neighbour to the right" ;
  rdfs:subPropertyOf geo:sfTouches ;
.
apo:hasNeighbourUp
  a owl:ObjectProperty ;
  rdfs:label "has neighbour upward" ;
  rdfs:subPropertyOf geo:sfTouches ;
.
auspix:Agg_1
  a apo:CellAggregate ;
  dcterms:identifier "Agg_1" ;
  rdfs:member apo:R7828 ;
  rdfs:member apo:R78520 ;
  rdfs:member apo:R78521 ;
  rdfs:member apo:R78522 ;
  rdfs:member apo:R78523 ;
.
auspix:R7852
  a apo:Cell ;
  apo:downNeighbour apo:R7855 ;
  apo:leftNeighbour apo:R7851 ;
  apo:rightNeighbour apo:R8630 ;
  apo:upNeighbour apo:R7828 ;
  geox:centroid "POINT (149.44444444444443 -35.23915910922053)"^^geo:wktLiteral ;
  geox:hasAreaM2 [
      data:value "12971551595"^^xsd:decimal ;
    ] ;
  dcterms:identifier "R7852" ;
  geo:hasGeometry "POLYGON ((148.88888888888889 -34.663795228918765, 150.0 -34.663795228918765, 150.0 -35.81859718358464, 148.88888888888889 -35.81859718358464))"^^geo:wktLiteral ;
  geo:sfContains apo:R78520 ;
  geo:sfContains apo:R78521 ;
  geo:sfContains apo:R78522 ;
  geo:sfContains apo:R78523 ;
  geo:sfContains apo:R78524 ;
  geo:sfContains apo:R78525 ;
  geo:sfContains apo:R78526 ;
  geo:sfContains apo:R78527 ;
  geo:sfContains apo:R78528 ;
  geo:sfWithin apo:R785 ;
.
<https://orcid.org/0000-0002-3884-3420>
  a owl:NamedIndividual ;
  a sdo:Person ;
  sdo:affiliation <https://linked.data.gov.au/org/csiro> ;
  sdo:email "simon.cox@csiro.au"^^xsd:anyURI ;
  sdo:url "https://orcid.org/0000-0002-3884-3420"^^xsd:anyURI ;
  sdo:name "Simon J D Cox"@en ;
.
